code/tests/Hacl.Test.ECDSA.fst
@@ -14,18 +14,33 @@ module B = LowStar.Buffer
 #set-options "--fuel 0 --ifuel 0 --z3rlimit 100"
 
 noextract
-let vectors_tmp = List.Tot.map 
+let sigver_vectors_tmp = List.Tot.map 
   (fun x -> h x.msg, h x.qx, h x.qy, h x.r, h x.s, x.result)
-  test_vectors
+  sigver_vectors
 
-%splice[vectors_low] (lowstarize_toplevel "vectors_tmp" "vectors_low")
+#push-options "--lax"
+
+%splice[sigver_vectors_low] 
+  (lowstarize_toplevel "sigver_vectors_tmp" "sigver_vectors_low")
+
+noextract
+let siggen_vectors_tmp = List.Tot.map 
+  (fun x -> h x.msg', h x.d, h x.qx', h x.qy', h x.k, h x.r', h x.s')
+  siggen_vectors
+
+%splice[siggen_vectors_low] 
+  (lowstarize_toplevel "siggen_vectors_tmp" "siggen_vectors_low")
+
+#pop-options
 
 // Cheap alternative to friend Lib.IntTypes needed because Test.Lowstarize uses UInt8.t
 assume val declassify_uint8: squash (uint8 == UInt8.t)
 
 let vec8 = L.lbuffer UInt8.t
 
-let vector = vec8 & vec8 & vec8 & vec8 & vec8 & bool
+let sigver_vector = vec8 & vec8 & vec8 & vec8 & vec8 & bool
+
+let siggen_vector = vec8 & vec8 & vec8 & vec8 & vec8 & vec8 & vec8
 
 // This could replace TestLib.compare_and_print
 val compare_and_print: b1:B.buffer UInt8.t -> b2:B.buffer UInt8.t -> len:UInt32.t 
@@ -44,7 +59,7 @@ let compare_and_print b1 b2 len =
   pop_frame();
   b
 
-let test_one (vec:vector) : Stack unit (requires fun _ -> True) (ensures fun _ _ _ -> True) =
+let test_sigver (vec:sigver_vector) : Stack unit (requires fun _ -> True) (ensures fun _ _ _ -> True) =
   let max_msg_len = 0 in
   let LB msg_len msg, 
       LB qx_len qx, 
@@ -77,6 +92,128 @@ let test_one (vec:vector) : Stack unit (requires fun _ -> True) (ensures fun _ _
     pop_frame()
     end
 
+val reverse_inplace_state: n:size_nat -> i:size_nat{i <= n / 2} -> Type0
+let reverse_inplace_state n i = Lib.Sequence.lseq uint8 n
+
+noextract
+val reverse_inplace_inner: n:size_nat -> i:size_nat{i < n / 2}
+  -> reverse_inplace_state n i -> reverse_inplace_state n (i + 1)
+let reverse_inplace_inner n i s =
+  let open Lib.Sequence in
+  let tmp = s.[i] in
+  let s = s.[i] <- s.[n - i - 1] in
+  s.[n - i - 1] <- tmp
+
+noextract
+val reverse_inplace_spec: n:size_nat -> s:Lib.Sequence.lseq uint8 n -> Lib.Sequence.lseq uint8 n
+let reverse_inplace_spec n s =
+    Lib.LoopCombinators.repeat_gen (n / 2) (reverse_inplace_state n)
+      (reverse_inplace_inner n) s
+
+val reverse_inplace: n:size_t{0 < v n} -> a:Lib.Buffer.lbuffer uint8 n -> Stack unit
+  (requires fun h0 -> Lib.Buffer.live h0 a)
+  (ensures  fun h0 _ h1 ->
+    Lib.Buffer.modifies1 a h0 h1 /\ 
+    Lib.Buffer.as_seq h1 a == reverse_inplace_spec (v n) (Lib.Buffer.as_seq h0 a))
+
+let reverse_inplace n a =
+  let open Lib.Buffer in
+  push_frame();
+  let h0 = get() in
+  loop h0 (n /. size 2) (reverse_inplace_state (v n))
+    (fun h i -> as_seq h a)
+    (fun i -> loc a)
+    (fun h0 -> reverse_inplace_inner (v n))
+    (fun i ->
+      Lib.LoopCombinators.unfold_repeat_gen (v n / 2)
+        (reverse_inplace_state (v n))
+        (reverse_inplace_inner (v n)) 
+        (Lib.Buffer.as_seq h0 a) (v i);
+      let tmp = a.(i) in
+      a.(i) <- a.(n -! i -! size 1);
+      a.(n -! i -! size 1) <- tmp
+    );
+  pop_frame()
+
+
+let test_siggen (vec:siggen_vector) : Stack unit (requires fun _ -> True) (ensures fun _ _ _ -> True) =
+  // TODO: remove refinement in msg in signing
+  assert_norm (pow2 32 < pow2 61);
+  let max_msg_len = 0 in
+  let LB msg_len msg,
+      LB d_len d,
+      LB qx_len qx, 
+      LB qy_len qy,
+      LB k_len k,
+      LB r_len r, 
+      LB s_len s = vec
+  in
+  B.recall msg;
+  B.recall d;
+  B.recall qx;
+  B.recall qy;
+  B.recall k;
+  B.recall r;
+  B.recall s;
+
+  // We need to check this at runtime because Low*-ized vectors don't carry any refinements
+  if not (d_len = 32ul && qx_len = 32ul && qy_len = 32ul && k_len = 32ul && r_len = 32ul && s_len = 32ul)
+  then C.exit (-1l)
+  else
+    begin
+    push_frame();
+    let rs = B.alloca (u8 0) 64ul in
+    let qxy = B.alloca (u8 0) 64ul in
+    B.blit qx 0ul qxy 0ul 32ul;
+    B.blit qy 0ul qxy 32ul 32ul;
+
+    // TODO: signing uses wrong byte order; this is a temporary workaround.
+    reverse_inplace 32ul d;
+    reverse_inplace 32ul k;
+
+    // TODO: the disjointness condition of signing need to be weakened
+    assume (let open Lib.Buffer in
+      B.all_disjoint [loc #MUT rs; loc #MUT msg; loc #MUT d; loc #MUT k]);
+    let h = get() in
+    assume (
+      let d: Lib.Buffer.lbuffer uint8 32ul = d in
+      let k: Lib.Buffer.lbuffer uint8 32ul = k in
+      Lib.ByteSequence.nat_from_bytes_le (Lib.Buffer.as_seq h d) <
+        Hacl.Spec.ECDSAP256.Definition.prime_p256_order /\
+      Lib.ByteSequence.nat_from_bytes_le (Lib.Buffer.as_seq h k) <
+        Hacl.Spec.ECDSAP256.Definition.prime_p256_order);
+    let flag = ecdsa_p256_sha2_sign rs msg_len msg d k in
+    if Lib.RawIntTypes.u64_to_UInt64 flag = 0uL then 
+      begin
+      // TODO: signing uses wrong byte order; this is a temporary workaround.
+      reverse_inplace 32ul (B.sub rs 0ul 32ul);
+      reverse_inplace 32ul (B.sub rs 32ul 32ul);
+      
+      let okr = compare_and_print (B.sub rs 0ul 32ul) r 32ul in
+      let oks = compare_and_print (B.sub rs 32ul 32ul) s 32ul in
+      if okr && oks then
+        begin
+        let result = ecdsa_p256_sha2_verify_u8 msg_len msg qxy r s in
+        if not result then
+          begin
+          LowStar.Printf.(printf "FAIL: verification\n" done);
+          C.exit 1l
+          end
+        end
+      else 
+        begin
+        LowStar.Printf.(printf "FAIL: signing\n" done);
+        C.exit 1l
+        end
+      end
+    else 
+      begin
+      LowStar.Printf.(printf "FAIL: signing\n" done);
+      C.exit 1l
+      end;
+    pop_frame()
+    end
+
 
 inline_for_extraction noextract
 let test_many #a (label:C.String.t) 
@@ -96,7 +233,8 @@ let test_many #a (label:C.String.t)
   in
   C.Loops.for 0ul len (fun _ _ -> True) f
 
-let main () : St C.exit_code =
-  test_many C.String.(!$"[ECDSA]") test_one vectors_low;
-  C.EXIT_SUCCESS
 
+let main () : St C.exit_code =
+  test_many C.String.(!$"[ECDSA SigVer]") test_sigver sigver_vectors_low;
+  test_many C.String.(!$"[ECDSA SigGen]") test_siggen siggen_vectors_low;
+  C.EXIT_SUCCESS
